get stumped by a seemingly simple theorem

algorithm_design/Perm.v
@@ -1,6 +1,89 @@
-From Coq Require Import List Permutation.
+From Coq Require Import List Permutation Nat Datatypes PeanoNat.
+Import ListNotations.
 
-Check list.
+Fixpoint insert {X : Type} (pos : nat) (x : X) (l : list X) : list X :=
+  match pos with
+  | O => x :: l
+  | S pred => match l with
+              | h :: t => h :: insert pred x t
+              | [] => [x]
+              end
+  end.
+
+Fixpoint permute {X : Type} (swaps : list nat) (l : list X) : list X :=
+  match swaps, l with
+  | n :: swaps', h :: t => insert n h (permute swaps' t)
+  | [], [] => []
+  | [], h :: t => h :: t
+  | n :: swaps, [] => []
+  end.
+
+Definition swap_inserts (m n : nat) : nat * nat :=
+  match n <=? m with
+  | true => (n, m)
+  | false => ((S n), m)
+  end.
+
+Theorem insert_not_empty : forall X pos (x : X) l, ~ ([] = insert pos x l).
+Proof.
+  intros. destruct pos; destruct l; discriminate.
+Qed.
+
+Theorem insert_spec : forall X pos (x : X) l,
+    (insert pos x l) = (firstn pos l) ++ [x] ++ (skipn pos l).
+Proof.
+  Search (nat -> list _ -> list _). intros.
+  - induction pos.
+    * reflexivity.
+    * simpl. induction l.
+      + reflexivity.
+      + fold firstn in IHl. admit.
+Admitted.
+
+Theorem swap_inserts_swaps : forall X n0 n1 h0 h1 (t : list X),
+  insert (S n0) h0 (insert n1 h1 t) =
+  let (m0, m1) := swap_inserts n0 n1 in
+  insert m0 h1 (insert m1 h0 t).
+Proof.
+  intros. unfold swap_inserts. Search (Bool.reflect (?a <= ?b) (?a <=? ?b)).
+  destruct (Nat.leb_spec0 n1 n0) as [Smaller | Bigger].
+  - induction Smaller.
+    * remember (insert n1 h1 t) as Insert11.
+      remember (insert n1 h0 t) as Insert10.
+      destruct Insert11. exfalso.
+      apply (insert_not_empty _ _ _ _ HeqInsert11).
+      simpl. admit.
+    * admit.
+  - apply Compare_dec.not_le in Bigger.
+
+  
+
+Definition insert_to_permute (f : nat -> list nat -> list nat) := 
+ forall (X : Type) (i : nat) (s : list nat) (h : X) (t : list X),
+   insert i h (permute s t) = permute (f i s) (h :: t).
+
+Definition
+
+permute s (permute (i1 :: s1) (h :: t))
+
+permute (i0 :: i0' :: s0) (insert (S O) h (l :: ls))
+permute (i0 :: i0' :: s0) (l :: h :: ls)
+insert i0 l (permute (i0' :: s0) (h :: ls))
+insert i0 l (insert i0' h (permute s ls))
+insert i0'' h (insert i0' l (permute s ls))
+
+Theorem permute_cons_O_right : forall X i s0 s1 s' h (t : list X),
+  permute s0 (permute s1 t) = permute s' t ->
+  permute (i :: s0) (permute (O :: s1) (h :: t)) =
+  permute (i :: s') (h :: t).
+Proof.
+  intros. simpl. rewrite H. reflexivity.
+Qed.
+
+
+permute (i :: s0) (permute ((S pred) :: s1) (h :: t))
+permute (i :: s0) (insert (S pred) h (permute s1 t))
+
 
 Fixpoint inserts {X : Type} (x : X) (l s : list X) : Prop :=
   (s = List.cons x l) \/
